Refactor

examples/dot_fused.v
@@ -1,5 +1,5 @@
 Require Import Monad SkelLib Computation ZArith TypedTerm Program.
-Require Import Compiler Ext Extract Host CompilerProof LibTactics.
+Require Import Compiler Ext Extract Host CompilerProof Fusion LibTactics.
 Open Scope Z_scope.
 
 Require Import DepList.
@@ -14,12 +14,34 @@ Definition dot_fused_IR : AS (TZ :: TZ :: nil) TZ :=
   ) (
   ARet _ _ HFirst).
 
+Definition dot (xs ys : list Z) : comp (list Z)
+  := do! t <- mapM (fun xy => ret (fst xy * snd xy)) (zip xs ys) in
+     reduceM (fun x y => ret (x + y)) t.
+
+Definition dot_fused_GPGPU :
+  {p : GModule | @equivGC (Skel.TZ :: Skel.TZ :: nil) (Skel.TZ) dot p}.
+Proof.
+  unfold dot; simpl.
+  reifyFunc.
+  eapply equivIC_weaken.
+  { introv Heq; applys (>>simple_fusion_correct Heq).
+    repeat econstructor; simpl.
+    - intros; omega.
+    - intros; omega. }
+  unfold simple_fusion; simpl.
+  unfold fuse_f1, body_of_func1, lift_sexp; simpl.
+  apply compileOk.
+  repeat econstructor; simpl.
+  - intros; omega.
+  - intros; omega.
+Defined.
+
 Goal False.
   pose (asDenote _ _ dot_fused_IR) as D.
   simpl in D.
 Abort.
 
-Definition res := save_to_file (compile_prog 1024 24 dot_fused_IR) "./dot_fused.cu".
+Definition res := save_to_file (`dot_fused_GPGPU) "./dot_fused.cu".
 
 Cd "extracted".
 
